Show:
\begin{align*}
	\theta_{MLE} &= \argmax_\theta P(X=x|\theta) \\
	\Rightarrow 0 &= \frac{\di P}{\di \theta}(\theta_{MLE}) \\
	\Rightarrow 0 &= \frac{\di \log{P}}{\di \theta} (\theta_{MLE})
\end{align*}

\begin{align*}
	\log P(X=m|\theta) &= \log{\binom{N}{m}\theta^m (1-\theta)^{n-m}} \\
	&= \log{\binom{N}{m}}+ m \cdot \log{\theta} + (N-m) \cdot \log{(1-\theta)}
\end{align*}

\begin{align*}
0 &= \frac{\di}{\di \theta} ( \log{\binom{N}{m}}+ m \cdot \log{\theta} + (N-m) \cdot \log{(1-\theta)} ) \\
	&= m \cdot \frac{1}{\theta} + (N-m) \cdot \frac{1}{1-\theta} \cdot (-1) \\
	&= \frac{m}{\theta} - \frac{N-m}{1-\theta} \\
	\Leftrightarrow \frac{N-m}{1-\theta} &= \frac{m}{\theta} \\
	\Leftrightarrow \frac{N-m}{m} &= \frac{1-\theta}{\theta} \\
	\Leftrightarrow \frac{N-m}{m} &= \frac{1}{\theta} - 1 \\
	\Leftrightarrow \frac{N-m}{m} +1 &= \frac{1}{\theta} \\
	\Leftrightarrow \frac{N-m+m}{m}  &= \frac{1}{\theta} \\
	\Leftrightarrow \theta &= \frac{m}{N} \\
	\Rightarrow \theta_{MLE} &= \frac{|X=1|}{|X=1|+|X=0|} \
	\end{align*}



Formalized Problem: \\
$mean(P(\theta | D )) = \lambda * mean(p(\theta)) + (1-\lambda ) * \theta_{MLH} $ \\
$mean(Beta(a +|X=1|,b +|X=0| )) = \lambda * mean(Beta(a,b)) + (1-\lambda ) * \theta_{MLH} $ \\
$\frac{a+|X=1|}{a+|X=1|+b+|X=0|} = \lambda * \frac{a}{a+b} + (1-\lambda ) * \frac{|X=1|}{|X=1|+|X=0|} $ \\

With: $0\le \lambda \le 1$ \\

Solution:\\

\begin{align*}
&\frac{a+|X=1|}{a+|X=1|+b+|X=0|}  \\
&=\frac{a}{a+|X=1|+b+|X=0|} + \frac{|X=1|}{a+|X=1|+b+|X=0|}   \\
&=\frac{a}{a+b+|X=1|+|X=0|} + \frac{|X=1|}{|X=1|+|X=0|+a+b}   \\
&=\frac{a}{a+b*(1+\frac{|X=1|+|X=0|}{a+b}} + \frac{|X=1|}{|X=1|+|X=0|*(1+\frac{a+b}{|X=1|+|X=0|}}   \\
&=\frac{a}{a+b}*\frac{1}{1+\frac{|X=1|+|X=0|}{a+b}} + \frac{|X=1|}{|X=1|+|X=0|}*\frac{1}{(1+\frac{a+b}{|X=1|+|X=0|}}  \\
&=\frac{a}{a+b}*\frac{1}{1+\frac{|X=1|+|X=0|}{a+b}} + \frac{|X=1|}{|X=1|+|X=0|}*\frac{|X=1|+|X=0|}{(|X=1|+|X=0|+(a+b)}  \\
&=\frac{a}{a+b}*\frac{1}{1+\frac{|X=1|+|X=0|}{a+b}} + \frac{|X=1|}{|X=1|+|X=0|}*(\frac{|X=1|+|X=0|+a+b}{(|X=1|+|X=0|)+(a+b)}) \\ &-\frac{a+b}{(|X=1|+|X=0|+(a+b))}  \\
&=\frac{a}{a+b}*\frac{1}{1+\frac{|X=1|+|X=0|}{a+b}} + \frac{|X=1|}{|X=1|+|X=0|}*(1-\frac{a+b}{(|X=1|+|X=0|+(a+b))})  \\
&=\frac{a}{a+b}*\frac{1}{1+\frac{|X=1|+|X=0|}{a+b}} + \frac{|X=1|}{|X=1|+|X=0|}*(1-\frac{1}{(\frac{|X=1|+|X=0|}{a+b}+1)})  \\
\end{align*}
Insert: \\
\\
$\lambda = \frac{1}{1+\frac{|X=1|+|X=0|}{a+b}}$ \\
$ mean(P(\theta | D )) = \lambda * \frac{a}{a+b} + (1-\lambda ) * \frac{|X=1|}{|X=1|+|X=0|} $ \\

qed.
