$ P(\lambda | x) = \frac{P(X|\lambda) * P(\lambda)}{P(X)}$ \\
$ P(\lambda | x) = \frac{P(X|\lambda) * P(\lambda)}{\int_{0}^{\infty}(P(X|\lambda) * P(\lambda))d{\lambda}}$ \\

Step 1: \\

$\int_{0}^{\infty} P(\lambda) D{\lambda} = 1$\\
$\int_{0}^{\infty} Gamma(a,b) D{\lambda} = 1$\\
$\int_{0}^{\infty} \frac{b^a}{\Gamma(a)} * \lambda^{a-1} * e^{-b\lambda} D{\lambda} = 1$\\ 
$\frac{b^a}{\Gamma(a)} * \int_{0}^{\infty} \lambda^{a-1} * e^{-b\lambda} D{\lambda} = 1$\\
$\int_{0}^{\infty} \lambda^{a-1} * e^{-b\lambda} D{\lambda} = \frac{\Gamma(a)}{b^a}$\\

Step2: \\

$P(X) = \int_{0}^{\infty}(P(X|\lambda) * P(\lambda))d{\lambda} $ \\
$\int_{0}^{\infty}(P(X|\lambda) * Gamma(a,b) )d{\lambda} =$ \\
$\int_{0}^{\infty}\frac{e^{-\lambda} * \lambda^x}{x!} * \frac{b^a}{\Gamma(a)} * \lambda^{a-1} * e^{-b\lambda} )d{\lambda} =$ \\
$\frac{b^a}{\Gamma(a)*x!} \int_{0}^{\infty}e^{-\lambda} * \lambda^x * \lambda^{a-1} * e^{-b\lambda} )d{\lambda} =$\\

$\frac{b^a}{\Gamma(a)*x!} \int_{0}^{\infty} \lambda^{x+a-1} * e^{-(b+1)\lambda} )d{\lambda} =$\\
Applying Step1:\\
$\frac{b^a}{\Gamma(a)*x!} * \frac{\Gamma(x+a)}{(b+1)^{x+a}}$\\
Putting it together:\\
$ P(\lambda | x) = \frac{P(X|\lambda) * P(\lambda)}{P(X)}=$ \\
$\frac{\frac{e^{-\lambda} * \lambda^x}{x!} * \frac{b^a}{\Gamma(a)} * \lambda^{a-1} * e^{-b\lambda} }{\frac{b^a}{\Gamma(a)*x!} * \frac{\Gamma(x+a)}{(b+1)^{x+a}}} =$ \\

$\frac{\frac{b^a}{\Gamma(a)*x!} * {e^{-\lambda} * \lambda^x} * \lambda^{a-1} * e^{-b\lambda} }{\frac{b^a}{\Gamma(a)*x!} * \frac{\Gamma(x+a)}{(b+1)^{x+a}}} $ \\

$\frac{{e^{-\lambda} * \lambda^x} * \lambda^{a-1} * e^{-b\lambda} }{ \frac{\Gamma(x+a)}{(b+1)^{x+a}}} $ \\

${e^{-\lambda} * \lambda^x} * \lambda^{a-1} * e^{-b\lambda} * \frac{(b+1)^{x+a}}{\Gamma(x+a)} = $ \\ 
$\lambda^{a+x-1} * e^{-(b+1)\lambda} * \frac{(b+1)^{x+a}}{\Gamma(x+a)} = $ \\
%$\frac{(b+1)^{x+a}}{\Gamma(x+a)}*\lambda^{a+x-1} * e^{-(b+1)\lambda} = $ \\
$Gamma(a+x,b+1)$

Calculating Map: \\
$\frac{d}{d\lambda} P(\lambda | x)  = 0$

$\frac{d}{d\lambda} ln (P(\lambda | x))  = 0$
$\frac{d}{d\lambda} ln (P(\lambda | x))   = \frac{d}{d\lambda} ln(\frac{(b+1)^{x+a}}{\Gamma(x+a)}*\lambda^{a+x-1} * e^{-(b+1)\lambda}) = $ \\
$\frac{d}{d\lambda} ln(\frac{(b+1)^{x+a}}{\Gamma(x+a)})+ ln(\lambda^{a+x-1}) + ln(e^{-(b+1)\lambda}) = $ \\
$\frac{d}{d\lambda}(a+x-1)*ln(\lambda) + {-(b+1)\lambda} = $ \\
$(a+x-1)*\frac{1}{\lambda} + -(b+1)$ \\

$(a+x-1)*\frac{1}{\lambda} + -(b+1) = 0$ \\
$(a+x-1)*\frac{1}{\lambda} = (b+1)$ \\
$(a+x-1) = (b+1) \lambda$ \\
$\lambda = \frac{a+x+1}{b+1}$ \\
$\Theta_{MAP} = \frac{a+x+1}{b+1}$
