\subsection*{Basics}
$\lambda Trick:$ \\
$\sum_{i=0}^{n+1} {\lambda_i} = 1  \wedge \lambda'_i = \frac{\lambda_i}{(1-\lambda_{n+1})} \rightarrow \sum_{i=0}^{n} {\lambda'_i} = 1  $ \\ 
Definition Convex: \\ 
$\forall x_1, x_2  \forall t \in [0,1]$ $ f(tx_1 + (1-t) x_2) \leq t*f(x_1) +(1-t)*f(x_2) $
\subsection*{Induction}
\subsubsection*{Hypothese}
$ f(\sum_{i=0}^{n} {\lambda_i x_i} ) \leq \sum_{i=0}^{n} {\lambda_i f(x_i)} | \sum_{i=0}^{n} {\lambda_i} = 1 $
\subsubsection*{Induction Start}
$n = 1 \wedge \lambda_1 = 1 $ \\
$f(\lambda_1x_1) \leq \lambda_1 * f(x_1) $ \\
$f(1*x_1) \leq 1 * f(x_1) $ \\
$f(x_1) \leq f(x_1) $

\subsubsection*{Induction Step}

$ f(\sum_{i=0}^{n+1} {\lambda_i x_i} ) \leq \sum_{i=0}^{n+1} {\lambda_i f(x_i)}  $ \\
Steps:\\
$   f(\sum_{i=0}^{n+1} {\lambda_i x_i} )  = f(\sum_{i=0}^{n} {\lambda_i x_i} + \lambda_{n+1}x_{n+1} ) $\\
$f(\sum_{i=0}^{n} {\lambda_i x_i} + \lambda_{n+1}x_{n+1} ) = f((1-\lambda_{n+1}) \sum_{i=0}^{n} {\lambda'_i x_i} + \lambda_{n+1}x_{n+1} )  $\\
$f((1-\lambda_{n+1}) \sum_{i=0}^{n} {\lambda'_i x_i} + \lambda_{n+1}x_{n+1} ) \leq (1-\lambda_{n+1}) f(\sum_{i=0}^{n} {\lambda'_i x_i}) + \lambda_{n+1}f(x_{n+1})$\\ 
$(1-\lambda_{n+1}) f(\sum_{i=0}^{n} {\lambda'_i x_i}) + \lambda_{n+1}f(x_{n+1}) \leq (1-\lambda_{n+1}) \sum_{i=0}^{n} {\lambda'_i f(x_i)} + \lambda_{n+1}f(x_{n+1})$\\
$(1-\lambda_{n+1}) \sum_{i=0}^{n} {\lambda'_i f(x_i)} + \lambda_{n+1}f(x_{n+1}) = \sum_{i=0}^{n} {\lambda_i f(x_i)} + \lambda_{n+1}f(x_{n+1})$\\
 $\sum_{i=0}^{n} {\lambda_i f(x_i)} + \lambda_{n+1}f(x_{n+1})= \sum_{i=0}^{n+1} {\lambda_i f(x_i)}$
