\begin{align*}
	\forall x_1, x_2 \in X , \forall t \in [0,1] \\
	f(tx_1 + (1-t)x_2) \le tf(x_1) +(1-t)f(x_2) \and  \\
	g(tx_1 + (1-t)x_2) \le tg(x_1) +(1-t)g(x_2) \\
	==> h(tx_1 + (1-t)x_2) \le th(x_1) +(1-t)h(x_2) 
\end{align*}

\begin{align*}
h(tx_1 + (1-t)x_2) &= f(tx_1 + (1-t)x_2) + g(tx_1 + (1-t)x_2) \\
&\le tf(x_1) +(1-t)f(x_2) + g(tx_1 + (1-t)x_2) \\
&\le tf(x_1) +(1-t)f(x_2) + tg(x_1) +(1-t)g(x_2) \\
&= t(f(x_1) + g(x_1)) +(1-t)(f(x_2)+g(x_2))\\
&= th(x_1) +(1-t)h(x_2)
\end{align*}

\begin{align*}
\forall x_1, x_2 \in X , \forall t \in [0,1] \\
f(tx_1 + (1-t)x_2) \le tf(x_1) +(1-t)f(x_2) \and  \\
c \ge 0 \\
==> u(tx_1 + (1-t)x_2) \le tu(x_1) +(1-t)u(x_2) 
\end{align*}

\begin{align*}
u(tx_1 + (1-t)x_2) &\le tu(x_1) +(1-t)u(x_2)\\
c* f(tx_1 + (1-t)x_2) &\le t*c*f(x_1) +(1-t)*c*f(x_2)  |\text{using c $\ge$ 0}\\
f(tx_1 + (1-t)x_2) &\le t*f(x_1) +(1-t)*f(x_2)\\
\end{align*}
