To show for concave functions:
\begin{align*}
g'(t*\alpha+(1-t)*\alpha) &\le t*g'(\alpha)+(1-t)*g'(\alpha)  \\
-g(t*\alpha+(1-t)*\alpha) &\le t*-g(\alpha)+(1-t)*-g(\alpha) \\
g(t*\alpha_1+(1-t)*\alpha_2) &\ge t*g(\alpha_1)+(1-t)*g(\alpha_2) \\
\underset{x}{min} L(x,t*\alpha_1+(1-t)*\alpha_2) &\ge
t*\underset{x}{min} L(x,\alpha_1)+(1-t)*\underset{x}{min} L(x,\alpha_2)\\
\underset{x}{min} f_0(x) + \sum_{i=1}^{m}((t*\alpha_{1,i}+(1-t)*\alpha_{2,i}) f_i(x)) 
&\ge t*\underset{x}{min} f_0(x) + \sum_{i=1}^{m}(\alpha_{1,i} f_i(x))  +(1-t)* \underset{x}{min} f_0(x) + \sum_{i=1}^{m}(\alpha_{2,i} f_i(x))
\end{align*}

\begin{align*}
t*\underset{x}{min} f_0(x) + \sum_{i=1}^{m}(\alpha_{1,i} f_i(x))  +(1-t)* \underset{x}{min} f_0(x) + \sum_{i=1}^{m}(\alpha_{2,i} f_i(x)) \\
\le t*\underset{x}{min} f_0(x) + \sum_{i=1}^{m}(\alpha_{1,i} f_i(x))  +(1-t)*(f_0(x) + \sum_{i=1}^{m}(\alpha_{2,i} f_i(x))) \\
=\underset{x}{min} tf_0(x) + \sum_{i=1}^{m}(t\alpha_{1,i} f_i(x))  +(1-t)*f_0(x) + \sum_{i=1}^{m}((1-t)*\alpha_{2,i} f_i(x)) \\
=\underset{x}{min} f_0(x) + \sum_{i=1}^{m}(t\alpha_{1,i} f_i(x)) + \sum_{i=1}^{m}((1-t)*\alpha_{2,i} f_i(x)) \\
=\underset{x}{min} f_0(x) + \sum_{i=1}^{m}((t\alpha_{1,i}+(1-t)*\alpha_{2,i}) f_i(x)) 
\end{align*}