\begin{align*}
f_0'(x) &= 2x \\
f_1'(x) &= 2x-6
\end{align*}

\begin{align*}
0 &= \frac{\di g(\alpha)}{\di \alpha} \\
  &= f_0'(\frac{3 \alpha_1}{1+\alpha_1}) \cdot \frac{3(1+\alpha_1) - 3 \alpha_1}{(1+\alpha_1)^2} + f_1(\frac{3 \alpha_1}{1+\alpha_1}) + \alpha_1 f_1'(\frac{3 \alpha_1}{1+\alpha_1}) \cdot \frac{3(1+\alpha_1) - 3 \alpha_1}{(1+\alpha_1)^2} \\
  &= f_0'(\frac{3 \alpha_1}{1+\alpha_1}) \cdot \frac{3}{(1+\alpha_1)^2} + f_1(\frac{3 \alpha_1}{1+\alpha_1}) + \alpha_1 f_1'(\frac{3 \alpha_1}{1+\alpha_1}) \cdot \frac{3}{(1+\alpha_1)^2} \\
  &= 2 \cdot \frac{3 \alpha_1}{1+\alpha_1} \cdot \frac{3}{(1+\alpha_1)^2} + (\frac{3\alpha_1}{1+\alpha_1} - 2)(\frac{3\alpha_1}{1+\alpha_1}-4) + \alpha_1 (2 \cdot \frac{3\alpha_1}{1+\alpha_1}-6) \cdot \frac{3}{(1+\alpha_1)^2} \\
  &= 18 \alpha_1 + (1+\alpha_1)(3 \alpha_1 - 2-2\alpha_1)(3\alpha_1-4-4\alpha_1) + 9 \alpha_1 (2\alpha_1-2-2\alpha_1) \\
  &= 18 \alpha_1 + (1+\alpha_1)(\alpha_1-2)(-\alpha_1-4) - 18 \alpha_1 \\
  &= (\alpha_1+1)(\alpha_1-2)(\alpha_1+4)
\end{align*}

\[ \Rightarrow \quad \alpha_1 = -1 \quad \lor \quad \alpha_1 = 2 \quad \lor \quad \alpha_1 = -4 \]

\begin{align*}
0 \leq \alpha^* \quad \Rightarrow \quad & \alpha^* = 2 \\
\Rightarrow \quad & g(\alpha^*) = 5
\end{align*}

